Grow-only_set/App.fst
@@ -2,17 +2,22 @@ module App
 
 open FStar.Seq
 open FStar.Ghost
+module L = FStar.List.Tot
 
-#set-options "--query_stats"
-
+let rec unique_s (l:list nat) =
+  match l with
+  |[] -> true
+  |id::xs -> not (L.mem id xs) && unique_s xs
+  
 // the concrete state type
-// e.g. for the increment only counter (icounter), concrete_st = nat
-type concrete_st = nat
+// It is a list of unique elements
+type concrete_st = l:list nat{unique_s l}
 
 //initial state
-let init_st = 0
+let init_st = []
 
-let eq (a b:concrete_st) = a == b
+let eq (a b:concrete_st) =
+  (forall e. L.mem e a <==> L.mem e b)
 
 let symmetric (a b:concrete_st) 
   : Lemma (requires eq a b)
@@ -27,14 +32,15 @@ let eq_is_equiv (a b:concrete_st)
           (ensures eq a b) = ()
           
 // operation type
-// (the only operation is increment, so unit is fine)
-type op_t = unit
+// (the only operation is Add, so nat is fine)
+type op_t = nat
 
 // concrete do pre-condition
 let concrete_do_pre _ _ = true
 
 // apply an operation to a state
-let do (s:concrete_st) (op:log_entry{concrete_do_pre s op}) : concrete_st = s + 1
+let do (s:concrete_st) (op:log_entry) : (r:concrete_st{(forall e. L.mem e r <==> L.mem e s \/ e = snd op)}) = 
+  if (L.mem (snd op) s) then s else (snd op)::s
 
 let lem_do (a b:concrete_st) (op:log_entry)
    : Lemma (requires concrete_do_pre a op /\ eq a b)
@@ -44,13 +50,14 @@ let lem_do (a b:concrete_st) (op:log_entry)
 //// Sequential implementation //////
 
 // the concrete state 
-type concrete_st_s = nat
+type concrete_st_s = l:list nat{unique_s l}
 
 // init state 
-let init_st_s = 0
+let init_st_s = []
 
 // apply an operation to a state 
-let do_s (s:concrete_st_s) (op:log_entry) : concrete_st_s = s + 1
+let do_s (s:concrete_st_s) (op:log_entry) : concrete_st_s = 
+  if (L.mem (snd op) s) then s else (snd op)::s
 
 //equivalence relation between the concrete states of sequential type and MRDT
 let eq_sm (st_s:concrete_st_s) (st:concrete_st) = st_s == st
@@ -67,34 +74,49 @@ let do_eq (st_s:concrete_st_s) (st:concrete_st) (op:log_entry)
 
 ////////////////////////////////////////////////////////////////
 
+let rec mem_ele (e:nat) (l:log) : Tot bool (decreases length l) =
+  match length l with
+  |0 -> false
+  |_ -> snd (head l) = e || mem_ele e (tail l)
+
 let rec lem_foldl (s:concrete_st) (l:log)
   : Lemma (requires foldl_prop s l)
-          (ensures (seq_foldl s l = s + length l) /\
-                   (length l > 0 ==> (foldl_prop s (fst (un_snoc l)) /\
-                                     seq_foldl s l = seq_foldl s (fst (un_snoc l)) + 1)))
+          (ensures (length l = 0 ==> s = seq_foldl s l) /\
+                   (forall e. L.mem e (seq_foldl s l) <==> L.mem e s \/ mem_ele e l))
           (decreases length l)
   = match length l with
     |0 -> ()
     |_ -> lem_foldl (do s (head l)) (tail l)
-    
+
 //conflict resolution
-let resolve_conflict (x y:log_entry) : (l:log{length l > 0 /\ last l = y}) =
+let resolve_conflict (x y:log_entry) : log =
   cons x (cons y empty)
 
 let resolve_conflict_prop (x y:log_entry)
   : Lemma (requires fst x <> fst y)
           (ensures last (resolve_conflict x y) <> x)
   = ()
-
+  
 // concrete merge pre-condition
-let concrete_merge_pre lca a b : prop
-  = a >= lca /\ b >= lca
+let concrete_merge_pre lca a b : prop = 
+  (forall e. L.mem e lca ==> L.mem e a /\ L.mem e b)
 
 // concrete merge operation
-let concrete_merge (lca:concrete_st) (s1:concrete_st) (s2:concrete_st{concrete_merge_pre lca s1 s2}) 
-  : concrete_st = s1 + s2 - lca
+let rec concrete_merge1 (lca:concrete_st) (s1:concrete_st) (s2:concrete_st) 
+  : Pure concrete_st (requires concrete_merge_pre lca s1 s2)
+                     (ensures (fun r -> (forall e. L.mem e r <==> L.mem e s1 \/ L.mem e s2))) 
+                     (decreases %[lca;s1;s2]) =
+  match lca, s1, s2 with
+  |[],[],[] -> []
+  |x::xs,_,_ -> concrete_merge1 xs s1 s2
+  |[],x::xs,_ -> if L.mem x s2 then concrete_merge1 [] xs s2 else x::(concrete_merge1 [] xs s2)
+  |[],[],x::xs -> x::concrete_merge1 [] [] xs
 
-#push-options "--z3rlimit 100"
+let concrete_merge (lca:concrete_st) (s1:concrete_st) (s2:concrete_st{concrete_merge_pre lca s1 s2})
+  : (r:concrete_st{(forall e. L.mem e r <==> L.mem e lca \/ L.mem e s1 \/ L.mem e s2)})=
+  concrete_merge1 lca s1 s2
+                    
+#push-options "--z3rlimit 200"
 let merge_inv_prop (lca s1 s2:st)
   : Lemma (requires is_prefix (ops_of lca) (ops_of s1) /\
                     is_prefix (ops_of lca) (ops_of s2) /\
@@ -110,40 +132,72 @@ let merge_inv_prop (lca s1 s2:st)
                       concrete_merge_pre (v_of lca) (v_of (inverse_st s1)) (v_of s2)) /\
                     (last (resolve_conflict last1 last2) <> last1 ==>
                       concrete_merge_pre (v_of lca) (v_of s1) (v_of (inverse_st s2))))) =
-  lem_foldl init_st (ops_of lca); 
+  let _, last1 = un_snoc (ops_of s1) in
+  let _, last2 = un_snoc (ops_of s2) in
+  lastop_neq (ops_of lca) (ops_of s1) (ops_of s2);
+  resolve_conflict_prop last1 last2;
   lem_foldl init_st (ops_of s1);
-  lem_foldl init_st (ops_of (inverse_st s2))
-                      
+  lem_foldl init_st (ops_of (inverse_st s2));
+  lem_inverse (ops_of lca) (ops_of s2);
+  split_prefix init_st (ops_of lca) (ops_of (inverse_st s2));
+  split_prefix init_st (ops_of lca) (ops_of s1);
+  lem_foldl (v_of lca) (diff (ops_of (inverse_st s2)) (ops_of lca));
+  lem_foldl (v_of lca) (diff (ops_of s1) (ops_of lca))
+
 let linearizable_s1_0 (lca s1 s2:st)
   : Lemma 
-      (requires concrete_merge_pre (v_of lca) (v_of s1) (v_of s2) /\
-                is_prefix (ops_of lca) (ops_of s1) /\
+      (requires is_prefix (ops_of lca) (ops_of s1) /\
                 is_prefix (ops_of lca) (ops_of s2) /\
                 ops_of s1 = ops_of lca /\
+                concrete_merge_pre (v_of lca) (v_of s1) (v_of s2) /\
                 (forall id id1. mem_id id (ops_of lca) /\ mem_id id1 (diff (ops_of s1) (ops_of lca)) ==> lt id id1) /\
                 (forall id id1. mem_id id (ops_of lca) /\ mem_id id1 (diff (ops_of s2) (ops_of lca)) ==> lt id id1) /\
-                (forall id. mem_id id (diff (ops_of s1) (ops_of lca)) ==> not (mem_id id (diff (ops_of s2) (ops_of lca)))) /\
                 foldl_prop (v_of lca) (diff (ops_of s2) (ops_of lca)))
-      (ensures v_of s2 == concrete_merge (v_of lca) (v_of s1) (v_of s2)) =
-  lem_foldl init_st (ops_of s2)
-
+      (ensures eq (v_of s2) (concrete_merge (v_of lca) (v_of s1) (v_of s2))) =
+  ()
+  
 let linearizable_s2_0 (lca s1 s2:st)
   : Lemma 
-      (requires concrete_merge_pre (v_of lca) (v_of s1) (v_of s2) /\
-                is_prefix (ops_of lca) (ops_of s1) /\
+      (requires is_prefix (ops_of lca) (ops_of s1) /\
                 is_prefix (ops_of lca) (ops_of s2) /\
                 Seq.length (ops_of s1) > Seq.length (ops_of lca) /\
                 ops_of s2 = ops_of lca /\
+                concrete_merge_pre (v_of lca) (v_of s1) (v_of s2) /\
                 (forall id id1. mem_id id (ops_of lca) /\ mem_id id1 (diff (ops_of s1) (ops_of lca)) ==> lt id id1) /\
                 (forall id id1. mem_id id (ops_of lca) /\ mem_id id1 (diff (ops_of s2) (ops_of lca)) ==> lt id id1) /\
-                (forall id. mem_id id (diff (ops_of s1) (ops_of lca)) ==> not (mem_id id (diff (ops_of s2) (ops_of lca)))) /\
                 foldl_prop (v_of lca) (diff (ops_of s1) (ops_of lca)))
-      (ensures v_of s1 == concrete_merge (v_of lca) (v_of s1) (v_of s2)) =
-  lem_foldl init_st (ops_of s1)
+      (ensures eq (v_of s1) (concrete_merge (v_of lca) (v_of s1) (v_of s2))) =
+  ()
 
-let lem_add (lca s1 s2:nat)
-  : Lemma (ensures s1 + (s2 - 1) - lca + 1 = s1 + s2 - lca)
-  = ()
+let linearizable_s2_gt0 (lca s1 s2:st)
+  : Lemma (requires is_prefix (ops_of lca) (ops_of s1) /\
+                    is_prefix (ops_of lca) (ops_of s2) /\
+                    Seq.length (ops_of s1) > Seq.length (ops_of lca) /\ 
+                    Seq.length (ops_of s2) > Seq.length (ops_of lca) /\
+                    is_prefix (ops_of lca) (ops_of (inverse_st s2)) /\
+                    concrete_merge_pre (v_of lca) (v_of s1) (v_of s2) /\
+                    concrete_merge_pre (v_of lca) (v_of s1) (v_of (inverse_st s2)) /\
+                    (forall id id1. mem_id id (ops_of lca) /\ mem_id id1 (diff (ops_of s1) (ops_of lca)) ==> lt id id1) /\
+                    (forall id id1. mem_id id (ops_of lca) /\ mem_id id1 (diff (ops_of s2) (ops_of lca)) ==> lt id id1) /\
+                    (forall id. mem_id id (diff (ops_of s1) (ops_of lca)) ==> not (mem_id id (diff (ops_of s2) (ops_of lca)))) /\
+                    (let _, last1 = un_snoc (ops_of s1) in
+                     let _, last2 = un_snoc (ops_of s2) in
+                     last (resolve_conflict last1 last2) <> last1))
+          (ensures (let _, last2 = un_snoc (ops_of s2) in
+                   concrete_do_pre (concrete_merge (v_of lca) (v_of s1) (v_of (inverse_st s2))) last2 /\
+                   eq (concrete_merge (v_of lca) (v_of s1) (v_of s2))
+                      (do (concrete_merge (v_of lca) (v_of s1) (v_of (inverse_st s2))) last2))) =
+  let _, last1 = un_snoc (ops_of s1) in
+  let p2, last2 = un_snoc (ops_of s2) in
+  inverse_helper init_st p2 last2;
+  assert (concrete_do_pre (concrete_merge (v_of lca) (v_of s1) (v_of (inverse_st s2))) last2); 
+  assert (forall e. L.mem e (concrete_merge (v_of lca) (v_of s1) (v_of s2)) <==>
+               L.mem e (concrete_merge (v_of lca) (v_of s1) (v_of (inverse_st s2))) \/ e = snd last2);
+  assert (forall e. L.mem e (do (concrete_merge (v_of lca) (v_of s1) (v_of (inverse_st s2))) last2) <==>
+               L.mem e (concrete_merge (v_of lca) (v_of s1) (v_of (inverse_st s2))) \/ e = snd last2);
+  assert (forall e. L.mem e (concrete_merge (v_of lca) (v_of s1) (v_of s2)) <==>
+               L.mem e (do (concrete_merge (v_of lca) (v_of s1) (v_of (inverse_st s2))) last2));
+  ()
 
 let linearizable_gt0 (lca s1 s2:st)
   : Lemma (requires is_prefix (ops_of lca) (ops_of s1) /\
@@ -166,24 +220,23 @@ let linearizable_gt0 (lca s1 s2:st)
                     let _, last2 = un_snoc (ops_of s2) in
                     (last (resolve_conflict last1 last2) = last1 ==>
                       concrete_do_pre (concrete_merge (v_of lca) (v_of (inverse_st s1)) (v_of s2)) last1 /\
-                      (concrete_merge (v_of lca) (v_of s1) (v_of s2) ==
-                      do (concrete_merge (v_of lca) (v_of (inverse_st s1)) (v_of s2)) last1)) /\
+                      eq (do (concrete_merge (v_of lca) (v_of (inverse_st s1)) (v_of s2)) last1)
+                         (concrete_merge (v_of lca) (v_of s1) (v_of s2))) /\
                     (last (resolve_conflict last1 last2) <> last1 ==>
                       concrete_do_pre (concrete_merge (v_of lca) (v_of s1) (v_of (inverse_st s2))) last2 /\
-                      (concrete_merge (v_of lca) (v_of s1) (v_of s2) ==
-                      do (concrete_merge (v_of lca) (v_of s1) (v_of (inverse_st s2))) last2)))) =
+                      eq (do (concrete_merge (v_of lca) (v_of s1) (v_of (inverse_st s2))) last2)
+                         (concrete_merge (v_of lca) (v_of s1) (v_of s2))))) =
   let _,last1 = un_snoc (ops_of s1) in
-  let _,last2 = un_snoc (ops_of s2) in
+  let p2,last2 = un_snoc (ops_of s2) in
   lastop_neq (ops_of lca) (ops_of s1) (ops_of s2);
   resolve_conflict_prop last1 last2;
-  assert (concrete_do_pre (concrete_merge (v_of lca) (v_of s1) (v_of (inverse_st s2))) last2);
-  lem_add (v_of lca) (v_of s1) (v_of s2)
+  linearizable_s2_gt0 lca s1 s2
 
 let convergence (lca s1 s2 s1':concrete_st) (o:log_entry)
   : Lemma (requires concrete_merge_pre lca s1 s2 /\
                     concrete_merge_pre lca s1' s2 /\
-                    concrete_do_pre s1 o /\ s1' == do s1 o /\
+                    concrete_do_pre s1 o /\ eq s1' (do s1 o) /\
                     concrete_merge_pre s1 (concrete_merge lca s1 s2) s1')
-          (ensures concrete_merge lca s1' s2 == concrete_merge s1 (concrete_merge lca s1 s2) s1') 
-  = ()
-#pop-options
+          (ensures eq (concrete_merge lca s1' s2) (concrete_merge s1 (concrete_merge lca s1 s2) s1')) = ()
+#pop-options 
+
